Verified the merge function of the leftist heap.

examples/miniML/okasaki-examples/LeftistHeapScript.sml
@@ -9,27 +9,33 @@ val cases_on = Cases_on;
 val every_case_tac = BasicProvers.EVERY_CASE_TAC;
 val full_case_tac = BasicProvers.FULL_CASE_TAC;
 
+val WeakLinearOrder_neg = Q.prove (
+`!leq x y. WeakLinearOrder leq ⇒ (~leq x y = leq y x ∧ x ≠ y)`,
+metis_tac [WeakLinearOrder, WeakOrder, trichotomous, reflexive_def,
+           antisymmetric_def]);
+
 val _ = new_theory "LeftistHeap"
 
 val _ = Hol_datatype `
-heaps = Empty | Node of num => 'a => heaps => heaps`;
+heap = Empty | Node of num => 'a => heap => heap`;
 
 val leftist_heap_to_bag_def = Define `
 (leftist_heap_to_bag Empty = {||}) ∧
 (leftist_heap_to_bag (Node _ x h1 h2) =
   BAG_INSERT x (BAG_UNION (leftist_heap_to_bag h1) (leftist_heap_to_bag h2)))`;
 
+val rank_def = Define `
+(rank Empty = 0) ∧
+(rank (Node r _ _ _) = r)`;
+
 val leftist_heap_ok_def = Define `
 (leftist_heap_ok leq Empty = T) ∧
 (leftist_heap_ok leq (Node _ x h1 h2) = 
   leftist_heap_ok leq h1 ∧
   leftist_heap_ok leq h2 ∧
-  (* OTHER STUFF *)
-  T)`;
-
-val rank_def = Define `
-(rank Empty = 0) ∧
-(rank (Node r _ _ _) = r)`;
+  BAG_EVERY (\y. leq x y) (leftist_heap_to_bag h1) ∧
+  BAG_EVERY (\y. leq x y) (leftist_heap_to_bag h2) ∧
+  rank h1 ≥ rank h2)`;
 
 val make_node_def = Define `
 make_node x a b =
@@ -46,13 +52,15 @@ val is_empty = Define `
 (is_empty _ = F)`;
 
 val merge_def = Define `
-(merge leq h1 Empty = h1) ∧
-(merge leq Empty h2 = h2) ∧
+(merge leq h Empty = h) ∧
+(merge leq Empty h = h) ∧
 (merge leq (Node n1 x a1 b1) (Node n2 y a2 b2) =
   if leq x y then
     make_node x a1 (merge leq b1 (Node n2 y a2 b2))
   else 
     make_node y a2 (merge leq (Node n1 x a1 b1) b2))`;
+
+val merge_ind = fetch "-" "merge_ind"
 
 val insert_def = Define `
 insert leq x h = merge leq (Node 1 x Empty Empty) h`;
@@ -62,5 +70,42 @@ find_min (Node _ x _ _) = x`;
   
 val delete_min_def = Define `
 delete_min leq _ x a b = merge leq a b`;
+
+val leftist_heap_merge_bag = Q.store_thm ("leftist_heap_merge_bag",
+`!leq h1 h2.
+  leftist_heap_to_bag (merge leq h1 h2) = 
+  BAG_UNION (leftist_heap_to_bag h1) (leftist_heap_to_bag h2)`,
+HO_MATCH_MP_TAC merge_ind >>
+srw_tac [BAG_ss] 
+        [merge_def, leftist_heap_to_bag_def, make_node_def, BAG_INSERT_UNION]);
+
+val leftist_heap_merge_ok = Q.store_thm ("leftist_heap_merge_ok",
+`!leq h1 h2. 
+  WeakLinearOrder leq ∧
+  leftist_heap_ok leq h1 ∧ 
+  leftist_heap_ok leq h2 
+  ⇒ 
+  leftist_heap_ok leq (merge leq h1 h2)`,
+HO_MATCH_MP_TAC merge_ind >>
+rw [merge_def, leftist_heap_ok_def, make_node_def, leftist_heap_merge_bag] >>
+rw [leftist_heap_to_bag_def] >|
+[metis_tac [BAG_EVERY, WeakLinearOrder, WeakOrder, transitive_def],
+ metis_tac [BAG_EVERY, WeakLinearOrder, WeakOrder, transitive_def],
+ metis_tac [BAG_EVERY, WeakLinearOrder, WeakOrder, transitive_def],
+ metis_tac [BAG_EVERY, WeakLinearOrder, WeakOrder, transitive_def],
+ decide_tac,
+ metis_tac [BAG_EVERY, WeakLinearOrder, WeakOrder, transitive_def,
+            WeakLinearOrder_neg],
+ metis_tac [BAG_EVERY, WeakLinearOrder, WeakOrder, transitive_def,
+            WeakLinearOrder_neg],
+ metis_tac [BAG_EVERY, WeakLinearOrder, WeakOrder, transitive_def,
+            WeakLinearOrder_neg],
+ metis_tac [BAG_EVERY, WeakLinearOrder, WeakOrder, transitive_def,
+            WeakLinearOrder_neg],
+ metis_tac [BAG_EVERY, WeakLinearOrder, WeakOrder, transitive_def,
+            WeakLinearOrder_neg],
+ metis_tac [BAG_EVERY, WeakLinearOrder, WeakOrder, transitive_def,
+            WeakLinearOrder_neg],
+ decide_tac]);
 
 val _ = export_theory ();
